\section{A Simple Induction Problem}

First, let's show the base case.\\
\\
\textbf{Base Case:} Consider $a_0 \leq 1$. We know that $a_0 \leq 2^0$, which proves the base case.\\
\\
\textbf{Hypothesis:} Assume that the proposition holds true for all $n < N$ where $N \in \mathbb{N}$ such that
$$
a_n \leq 2^n \text{ for all } n \leq N
$$
\textbf{Inductive Step:} Now, consider the term $a_{N+1}$. By the limitation on $a_N$, we know that
$$
a_{N+1} \leq \sum_{n=0}^N a_n = a_0 + a_1 + a_2 + \cdots + a_{N-1} + a_N
$$
Since we have the bound (via hypothesis), we can say that.
\begin{align*}
    a_{N+1} &\leq a_0 + a_1 + a_2 + \cdots + a_{N-1} + a_N\\
    &\leq 2^0 + 2^1 + 2^2 + \cdots + 2^{N-1} + 2^{N} \\
    &= 2^{N+1} - 1 \\
    &\leq 2^{N+1}
\end{align*}
This concludes the proof.

